Дано $f(x)$, $g(x)$ и $\exists f'(x),\ g'(x)$

$$\begin{align}
&1.\ (k(f(x)))'=\lim_{ \Delta x \to 0} \frac{kf(x+\Delta x)-kf(x)}{\Delta x}=kf'(x) \\
&2.\ (f(x)\pm g(x))'=\lim_{ \Delta x \to 0} \frac{f(x+\Delta x)\pm g(x+\Delta x)-f(x)-g(x)}{\Delta x} =\\
&=\lim_{ \Delta x \to 0} \frac{f(x+\Delta x)-f(x)}{\Delta x}\pm\lim_{ \Delta x \to 0} \frac{g(x+\Delta x)-g(x)}{\Delta x}=f'(x)\pm g'(x) \\
&3. \ (f(x)g(x))'=\lim_{ \Delta x \to 0} \frac{f(x+\Delta x) g(x+\Delta x)-f(x)g(x)}{\Delta x} =\\
&=\lim_{ \Delta x \to 0} \frac{f(x+\Delta x) g(x+\Delta x)-f(x)g(x+\Delta x)+f(x)g(x+\delta x)-f(x)g(x)}{\Delta x}= \\
&=\lim_{ \Delta x \to 0} \frac{f(x+\Delta x)-f(x)}{\Delta x}\cdot g(x+\Delta x)+f(x)\cdot\lim_{ \Delta x \to 0} \frac{g(x+\Delta x)-g(x)}{\Delta x}= \\
&=f'(x)g(x)+f(x)g'(x) \\
&4.\ \left( \frac{f(x)}{g(x)} \right)'=\lim_{ \Delta x \to 0} \frac{\frac{f(x+\Delta x)}{g(x+\Delta x)}-\frac{f(x)}{g(x)}}{\Delta x}=\lim_{ \Delta x \to 0} \frac{f(x+\Delta x) g(x)-f(x)g(x+\Delta x)}{g(x+\Delta x)g(x)\Delta x} = \\
&=\lim_{ \Delta x \to 0} \frac{1}{g(x+\Delta x)g(x)} \cdot\lim_{ \Delta x \to 0} \frac{f(x+\Delta x) g(x)-f(x)g(x)+f(x)g(x)-f(x)g(x+\Delta x)}{\Delta x}= \\
&=\frac{1}{g^{2}}(x)\cdot \left(g(x)\cdot\lim_{ \Delta x \to 0} \frac{f(x+\Delta x)-f(x)}{\Delta x}-f(x)\cdot \lim_{ \Delta x \to 0} \frac{g(x+\Delta x)-g(x)}{\Delta x} \right)= \\
&= \frac{f'(x)g(x)-f(x)g'(x)}{g^{2}(x)}
\end{align}$$
